theories/type_systems/stlc_extended_sol/types.v
@@ -139,7 +139,7 @@ Lemma canonical_values_arr Gamma e A B :
   is_val e ->
   exists x e', e = (lam: x, e')%E.
 Proof.
-  intros He [v ->]. inversion He; destruct v; simplify_eq; by eauto.
+  inversion 1; simplify_eq; by eauto.
 Qed.
 
 Lemma canonical_values_int Gamma e :
@@ -147,7 +147,7 @@ Lemma canonical_values_int Gamma e :
   is_val e ->
   exists n: Z, e = n.
 Proof.
-  intros He [v ->]. inversion He; destruct v; simplify_eq; by eauto.
+  inversion 1; simplify_eq; by eauto.
 Qed.
 
 (* new lemma *)
@@ -156,7 +156,7 @@ Lemma canonical_values_pair Gamma e A B :
   is_val e ->
   exists e1 e2, e = Pair e1 e2 /\ is_val e1 /\ is_val e2.
 Proof.
-  intros He [v ->]. inversion He; destruct v; simplify_eq; by eauto 10.
+  inversion 1; simplify_eq; by eauto 10.
 Qed.
 
 (** Definition 6 *)
@@ -178,7 +178,7 @@ Theorem type_progress e A :
     + eapply canonical_values_arr in Hty as (x & e & ->); last done.
       right. eexists.
       eapply base_contextual_step, BetaS; eauto.
-    + right. destruct H2 as [v ->].
+    + right. apply is_val_make_val in H2 as [v ->].
       destruct H1 as [e1' Hstep].
       eexists. eapply (fill_contextual_step [AppLCtx v]). done.
     + right. destruct H2 as [e2' H2].
@@ -187,7 +187,7 @@ Theorem type_progress e A :
     + right. eapply canonical_values_int in Hty1 as [n1 ->]; last done.
       eapply canonical_values_int in Hty2 as [n2 ->]; last done.
       eexists. eapply base_contextual_step. eapply PlusS; eauto.
-    + right. destruct H2 as [v ->].
+    + right. apply is_val_make_val in H2 as [v ->].
       destruct H1 as [e1' Hstep].
       eexists. eapply (fill_contextual_step [PlusLCtx v]). done.
     + right. destruct H2 as [e2' H2].
@@ -195,7 +195,7 @@ Theorem type_progress e A :
   (* New cases: *)
   - destruct (IH2 HeqGamma) as [H2|H2]; first destruct (IH1 HeqGamma) as [H1|H1].
     + left. by eauto.
-    + right. destruct H2 as (v2&->).
+    + right. apply is_val_make_val in H2 as (v2&->).
       destruct H1 as (e1'&H1). eexists.
       by eapply (fill_contextual_step [PairLCtx v2]).
     + right. destruct H2 as (e2'&H2). eexists.
